transformations/Moore2MealyALT/theorems/WFStable.v
@@ -1,0 +1,38 @@
+Require Moore2MealyALT.MooreSemantics.
+Require Moore2MealyALT.MealySemantics.
+Require Moore2MealyALT.Moore2Mealy.
+Require Moore2MealyALT.MooreWF.
+Require Moore2MealyALT.MealyWF.
+Require Moore2MealyALT.theorems.Elements.
+
+
+Lemma determinist_preserved m :
+  Moore.WF1 m ->
+  MooreWF.determinist m ->
+  MealyWF.determinist (Semantics.execute  Moore2Mealy.Moore2Mealy m).
+Proof.
+  intros WF_1 WF_2.
+  unfold MealyWF.determinist.
+  intros t1 t2 H1 H2 H3 H4.
+  apply Elements.transition_element_bw in H1 ; auto.
+  apply Elements.transition_element_bw in H2 ; auto.
+  destruct H1 as (mt1 & ? & ?).
+  destruct H2 as (mt2 & ? & ?).
+  specialize (WF_2 mt1 mt2 H H1).
+  unfold Elements.convert_transition in H0.
+  PropUtils.destruct_match H0 ; [ PropUtils.inj H0 | discriminate H0 ] ; simpl in *.
+  unfold Elements.convert_transition in H2.
+  PropUtils.destruct_match H2 ; [ PropUtils.inj H2 | discriminate H2 ] ; simpl in *.
+  specialize (WF_2 H3 H4).
+  subst.
+  rewrite Heqo in Heqo0 ; PropUtils.inj Heqo0. (* auto_unif *)
+  reflexivity.
+Qed.
+
+
+Lemma unique_names_preserved_fw : forall m,
+    MooreWF.unique_names m -> 
+    MealyWF.unique_names (Semantics.execute Moore2Mealy.Moore2Mealy m).
+Proof.
+  intros ; apply MealyWF.always_unique_names.
+Qed.
